fix: remove unused variable S in instances

Instances/Store.v
@@ -9,9 +9,9 @@ Require Import Classes.Monad.
 Section store_stateT_concrete. 
   Context (M : Type -> Type) `{M_monad : Monad M}.
 
-  Definition stateT_get (S : Type) := fun s : S => returnM (s, s).
+  Definition stateT_get := fun s : store => returnM (s, s).
 
-  Definition stateT_put (S : Type) := fun s : S => fun _ : S => returnM (tt, s).
+  Definition stateT_put := fun s : store => fun _ : store => returnM (tt, s).
 
   Definition retrieve_concrete (x : string) : StateT store M cvalue :=
     fun s : store => returnM (s x, s).
@@ -19,11 +19,11 @@ Section store_stateT_concrete.
   Definition update_concrete (x : string) (v : cvalue) : StateT store M store :=
     fun s : store => let s' := t_update s x v in returnM (s', s').
 
-  Global Instance store_stateT (S : Type) : 
+  Global Instance store_stateT : 
   Store store (StateT store M) cvalue :=
   {
-    get := stateT_get store;
-    put := stateT_put store;
+    get := stateT_get;
+    put := stateT_put;
     retrieve := retrieve_concrete;
     update := update_concrete;
   }.
@@ -32,19 +32,20 @@ End store_stateT_concrete.
 Section store_stateT_abstract.
   Context (M : Type -> Type) `{M_monad : Monad M}.
 
-  Definition get_abstract (S : Type) := fun s : S => returnM (s, s).
-  Definition put_abstract (S : Type) := fun s : S => fun _ : S => returnM (tt, s).
+  Definition get_abstract := fun s : abstract_store => returnM (s, s).
+  Definition put_abstract := fun s : abstract_store => 
+    fun _ : abstract_store => returnM (tt, s).
   Definition retrieve_abstract (x : string) : StateT abstract_store M avalue :=
     fun s : abstract_store => returnM (s x, s).
   Definition update_abstract (x : string) (v : avalue) : 
     StateT abstract_store M abstract_store :=
     fun s : abstract_store => let s' := t_update s x v in returnM (s', s').
 
-  Global Instance store_stateT_abstract (S : Type) : 
+  Global Instance store_stateT_abstract : 
     Store abstract_store (StateT abstract_store M) avalue :=
   {
-    get := get_abstract abstract_store;
-    put := put_abstract abstract_store;
+    get := get_abstract;
+    put := put_abstract;
     retrieve := retrieve_abstract;
     update := update_abstract;
   }.
